More work on closed proof; issue with matching up goose_ffiLocalGS's still

external/Goose/github_com/mit_pdos/gokv/simplepb/apps/closed.v
@@ -26,6 +26,8 @@ Definition kv_replica_main1: val :=
 
 Definition kv_replica_main2: val :=
   rec: "kv_replica_main2" <> :=
+    let: "x" := ref (zero_val uint64T) in
+    "x" <-[uint64T] #1;;
     kv64.Start #(str"kv.data") r2;;
     #().
 
